STLC/Semantics.v
@@ -38,6 +38,19 @@ Proof.
     subst;
     eauto.
 Qed.
+Hint Resolve simplto_preserves_evalto.
+
+Lemma simplto_preserves_diverge : forall e e',
+  simplto e e' ->
+  diverge e' ->
+  diverge e.
+Proof.
+  intros ? ? Hsimplto Hdiverge.
+  induction Hsimplto;
+    inversion Hdiverge;
+    subst;
+    eauto.
+Qed.
 
 Theorem simplto_multi_impl_evalto : forall e v,
   clos_refl_trans _ simplto e v ->
@@ -47,6 +60,5 @@ Proof.
   intros ? ? Hsimplto ?.
   apply clos_rt_rt1n in Hsimplto.
   Hint Constructors clos_refl_trans_1n.
-  Hint Resolve simplto_preserves_evalto.
   induction Hsimplto; eauto.
 Qed.
